CBS.h
@@ -14,6 +14,8 @@ typedef struct
 }
 CBS_cbs_t;
 
+bool CBS_cbs_skip(CBS_cbs_t *cbs, uint32_t num);
+
 bool CBS_cbs_get_u(CBS_cbs_t *cbs, uint32_t *out, uint32_t num);
 
 bool CBS_cbs_get_u8(CBS_cbs_t *cbs, uint8_t *out);
